src/simulation/Cert_ar.v
@@ -141,7 +141,7 @@ Hypothesis COMP_RPPO : dom_rel (⦗R⦘ ⨾ (Gdata ∪ Grfi ∪ Grmw)＊ ⨾ Grp
 Hypothesis TCCOH_rst_new_T : tc_coherent G sc (mkTC (C ∪₁ (E ∩₁ NTid_ thread)) I).
 
 Hypothesis S_in_W : S ⊆₁ W.
-Hypothesis RPPO_S : dom_rel ((Gdetour ∪ Grfe) ⨾ (Gdata ∪ Grfi ∪ Grmw)＊ ⨾ Grppo ⨾ ⦗S⦘) ⊆₁ I.
+Hypothesis RPPO_RMW_S : dom_rel ((Gdetour ∪ Grfe) ⨾ (Gdata ∪ Grfi ∪ Grmw)＊ ⨾ (Grppo ∪ Grmw) ⨾ ⦗S⦘) ⊆₁ I.
 Hypothesis ST_in_E : S ∩₁ Tid_ thread ⊆₁ E.
 Hypothesis I_in_S : I ⊆₁ S.
 Hypothesis W_ex_acq_in_I :GW_ex_acq ⊆₁ I.
