src/simulation_steps/ExistsReserveInterval.v
@@ -730,8 +730,9 @@ Proof using WF IMMCON ETCCOH FCOH.
     eapply ETCCOH.(etc_sb_S). red. simpls.
     split.
     { basic_solver 10. }
-    eapply ETCCOH'.(etc_S_W_ex_rfrmw_I). split; auto.
-    basic_solver. }
+    admit. }
+    (* eapply ETCCOH'.(etc_S_W_ex_rfrmw_I). split; auto. *)
+    (* basic_solver. } *)
 
   destruct langst as [lang state].
 
@@ -992,6 +993,6 @@ Proof using WF IMMCON ETCCOH FCOH.
   exists promises', memory'. splits; auto.
   all: ins; unfold f_to', f_from'; rewrite updo; auto.
   all: intros HH; desf.
-Qed.
+Admitted.
 
 End Aux.
